---
title: "SElshahawy_Assign14"
author: "Salma Elshahawy"
date: "5/8/2020"
output: 
  html_document:
    toc: true
    toc_float:
      collapsed: false
      smooth_scroll: true
    df_print: paged
  pdf_document:
    extra_dependencies: geometry
    keep_tex: yes
    latex_engine: xelatex
---

```{r setup, include=FALSE}
knitr::opts_chunk$set(echo = TRUE)
```

For each function, only consider its valid ranges as indicated in the notes when you are computing the Taylor Series expansion. Please submit your assignment as a R-Markdown document.

1. $f(x) =\frac{1}{(1-x)}$ 

When $1 - x = 0 \quad so \quad when \quad x = 1$ the function is not defined
Getting the first 5 terms in the tylor serier

$$f(x) = \frac{1}{(1-x)} \quad then \quad f(0) = 1$$

$$f'(x) = \frac{1}{(1-x)^2} \quad then \quad f'(0) = 1$$

$$f^2(x) = \frac{2}{(1-x)^3} \quad then \quad f^2(0) = 2$$
$$f^3(x) = \frac{6}{(1-x)^4} \quad then \quad f^3(0) = 6$$
$$f^4(x) = \frac{24}{(1-x)^5} \quad then \quad f^4(0) = 24$$
$$f^5(x) = \frac{120}{(1-x)^6} \quad then \quad f^5(0) = 120$$


We can apply the McClaurin Series formula 
$$1 + \frac{1}{1!} x^1 + \frac{2}{2!}x^2 + \frac{6}{3!}x^3 + \frac{24}{4!}x^4 + \frac{120}{5!}x^5 $$

To simplify, 
$$1 + x + x^2 + x^3 + x^4 + x^5$$

$$\sum_{n=0}^{\infty} x^n$$

2. $f(x)=e^x$

Derivatives and evaluation at $x = 0$
$$f^1(x)=e^x \quad then \quad f^1(0) = 1$$

$$f^2(x)=e^x \quad then \quad f^2(0) = 1$$

$$f^3(x)=e^x \quad then \quad f^3(0) = 1$$

$$f^4(x)=e^x \quad then \quad f^4(0) = 1$$

$$f^5(x)=e^x \quad then \quad f^5(0) = 1$$

$$1 + x + \frac{x^2}{2} + \frac{x^3}{6} + \frac{x^4}{24} + ... + \frac{x^n}{n!}$$
The summation formula 

$$\sum_{n=0}^{\infty} \frac{x^n}{n!}$$


3. $f(x)=ln(1+x)$

Derivatives and evaluation at $x = 0$

$$f^1(x) = \frac{1}{x+1} \quad then \quad f^1(0) = 1$$
$$f^2(x) = \frac{-1}{(x+1)^2} \quad then \quad f^2(0) = -1$$
$$f^3(x) = \frac{2}{(x+1)^3} \quad then \quad f^3(0) = 2$$
$$f^4(x) = \frac{-6}{(x+1)^4} \quad then \quad f^4(0) = -6$$
$$f^5(x) = \frac{24}{(x+1)^5} \quad then \quad f^5(0) = 24$$
after simplifying 
$$x - \frac{1}{2}x^2 + \frac{1}{3}x^3 - \frac{1}{4}x^4 + \frac{1}{5}x^5+ ... (-1)^{n+1}\frac{1}nx^n$$


$$\sum_{n=0}^{\infty} (-1)^{n+1}\frac{1}nx^n$$


